proof/props.v
@@ -1,0 +1,51 @@
+Require Import defs encoding thm bool int ptr.
+Require Import List.
+Import ListNotations.
+
+Lemma cheat {P: Prop} : P.
+Admitted.
+
+Lemma int_rt1 {ty: Ty} : rt1 ty.
+Proof.
+destruct ty.
+- apply bool_rt1.
+- apply int_rt1.
+- apply ptr_rt1.
+- apply cheat.
+- apply cheat.
+- apply cheat.
+Qed.
+
+Lemma int_rt2 {ty: Ty} : rt2 ty.
+Proof.
+destruct ty.
+- apply bool_rt2.
+- apply int_rt2.
+- apply cheat.
+- apply cheat.
+- apply cheat.
+- apply cheat.
+Qed.
+
+Lemma int_mono1 {ty: Ty} : mono1 ty.
+Proof.
+destruct ty.
+- apply bool_mono1.
+- apply int_mono1.
+- apply cheat.
+- apply cheat.
+- apply cheat.
+- apply cheat.
+Qed.
+
+Lemma int_mono2 {ty: Ty} : mono2 ty.
+Proof.
+destruct ty.
+- apply bool_mono2.
+- apply int_mono2.
+- apply cheat.
+- apply cheat.
+- apply cheat.
+- apply cheat.
+Qed.
+
